src/protocol/DNS.Protocol.Parser.EverParseAdapter.fst
@@ -116,24 +116,32 @@ let generated_dns_uncompressed_question_soa_answer_packet_validator
     rname_length
 
 let generated_dns_uncompressed_question_compressed_soa_mname_answer_packet_validator
-    qname_length rr_name_length rname_length =
+    qname_length rr_name_length rname_length mname_ptr_hi_value mname_ptr_lo_value =
   DNSProtocol.validate__dns_uncompressed_question_compressed_soa_mname_answer_packet
     qname_length
     rr_name_length
     rname_length
+    mname_ptr_hi_value
+    mname_ptr_lo_value
 
 let generated_dns_uncompressed_question_compressed_soa_rname_answer_packet_validator
-    qname_length rr_name_length mname_length =
+    qname_length rr_name_length mname_length rname_ptr_hi_value rname_ptr_lo_value =
   DNSProtocol.validate__dns_uncompressed_question_compressed_soa_rname_answer_packet
     qname_length
     rr_name_length
     mname_length
+    rname_ptr_hi_value
+    rname_ptr_lo_value
 
 let generated_dns_uncompressed_question_compressed_soa_answer_packet_validator
-    qname_length rr_name_length =
+    qname_length rr_name_length mname_ptr_hi_value mname_ptr_lo_value rname_ptr_hi_value rname_ptr_lo_value =
   DNSProtocol.validate__dns_uncompressed_question_compressed_soa_answer_packet
     qname_length
     rr_name_length
+    mname_ptr_hi_value
+    mname_ptr_lo_value
+    rname_ptr_hi_value
+    rname_ptr_lo_value
 
 let generated_dns_uncompressed_question_srv_answer_packet_validator
     qname_length rr_name_length target_name_length =
